Finish multi-rule programs

platform/tests/XmlTestDriver.v
@@ -1,1 +1,60 @@
-Require Export XmlProg.
+Require Import Bedrock Xml XmlProg.
+
+Module M.
+  Definition heapSize := (1024 * 1024)%N.
+
+  Definition ts := {| Name := "rpcs";
+    Address := ((heapSize + 50) * 4)%N;
+    Schema := "cmd" :: "a" :: "b" :: nil
+  |} :: nil.
+
+  Definition pr := Match
+    "rpc"/(
+      "cmd"/"frob"
+      & "mode"/$"mode"
+      & "args"/(
+        "string"/$"a";;
+        "string"/$"b"
+        )
+    )
+  Do
+    Write <*> "answer" </>
+      <*> "mode" </> $"mode" </>,
+      <*> "a" </> $"a" </>,
+      <*> "b" </> $"b" </>
+    </>;;
+    Insert "rpcs" ("frob", $"a", $"b");;
+    Write <*> "extra" </>
+      <*> "boring" </> "constant" </>,
+      <*> "B" </> $"b" </>
+    </>
+  end%program.
+
+  Theorem wellFormed : wf ts pr.
+    wf.
+  Qed.
+
+  Theorem notTooGreedy : (reserved pr <= 38)%nat.
+    compute; omega.
+  Qed.
+
+  Definition buf_size := 1024%N.
+
+  Theorem buf_size_lower : (buf_size >= 2)%N.
+    discriminate.
+  Qed.
+    
+  Theorem buf_size_upper : (buf_size * 4 < Npow2 32)%N.
+    reflexivity.
+  Qed.
+
+  Theorem ND : NoDup (Names ts).
+    NoDup.
+  Qed.
+
+  Theorem goodSchema : twfs ts.
+    goodSchema.
+  Qed.
+End M.
+
+Module E := Make(M).
