platform/NumOps.v
@@ -1,0 +1,70 @@
+Require Import AutoSep.
+
+
+Definition div4S := SPEC("n") reserving 1
+  Al m,
+  PRE[V] [| wordToNat (V "n") = m * 4 |]%nat
+  POST[R] [| R = m |].
+
+Definition m := bmodule "numops" {{
+  bfunction "div4"("n", "acc") [div4S]
+    "acc" <- 0;;
+
+    [Al m,
+      PRE[V] [| wordToNat (V "n") = m * 4 |]%nat
+      POST[R] [| R = natToW m ^+ V "acc" |] ]
+    While ("n" >= 4) {
+      "acc" <- "acc" + 1;;
+      "n" <- "n" - 4
+    };;
+
+    Return "acc"
+  end
+}}.
+
+Section ok.
+  Lemma use_pred : forall (w : W) n,
+    wordToNat w = n * 4
+    -> natToW 4 <= w
+    -> wordToNat w - 4 = (pred n) * 4.
+    intros.
+    nomega.
+  Qed.
+
+  Hint Immediate use_pred.
+
+  Lemma roundTrip_4 : wordToNat (natToW 4) = 4.
+    auto.
+  Qed.
+
+  Hint Rewrite roundTrip_4 : N.
+
+  Lemma cancel_pred : forall n m rv acc,
+    natToW 4 <= n
+    -> wordToNat n = m * 4
+    -> rv = natToW (pred m) ^+ (acc ^+ natToW 1)
+    -> rv = natToW m ^+ acc.
+    intros; subst.
+    rewrite Minus.pred_of_minus.
+    rewrite natToW_minus by nomega; words.
+  Qed.
+
+  Hint Immediate cancel_pred.
+
+  Lemma finish : forall rv acc n m,
+    rv = acc
+    -> n < natToW 4
+    -> wordToNat n = m * 4
+    -> rv = natToW m ^+ acc.
+    intros; subst.
+    assert (m0 = 0) by nomega.
+    words.
+  Qed.
+
+  Hint Immediate finish.
+  Hint Rewrite <- plus_n_O : sepFormula.
+
+  Theorem ok : moduleOk m.
+    vcgen; abstract (sep_auto; eauto).
+  Qed.
+End ok.
